More results on countability.

Quotients/Countable.v
@@ -10,4 +10,51 @@
     A type [A] is called countable if [option A] is a retract of the
     natural numbers. When [A] is inhabited, then it is equivalent to a
     retraction of [A] into the natural numbers, but this definition
-    also includes the empty set. *)
+    also includes the empty set.
+
+    Being countable is defined here as a type class, making the
+    hypothesis that the chosen retraction is unlikely to be tractable
+    (few of the instances defined in this file are) and that it's not
+    to be used in a real program, where some control will be
+    needed. *)
+
+Require Import FinSet.Quotients.Retract.
+Require Import Coq.NArith.NArith.
+
+
+Class Countable A := countable : Retract nat (option A).
+
+(** We also use an inhabitation type class, which will help avoid the
+    [option] type in our calculation. *)
+Class Inhabited A := inhabitant : A.
+
+Definition to_nat {A} {_:Countable A} {_:Inhabited A} : A -> nat :=
+  (retract_nat_inh countable inhabitant).(inj).
+Definition of_nat {A} {_:Countable A} {_:Inhabited A} : nat -> A :=
+  (retract_nat_inh countable inhabitant).(proj).
+
+Lemma nat_retract A {_:Countable A} {_:Inhabited A} : forall x, of_nat (to_nat x) = x.
+Proof.
+  intros *. unfold of_nat, to_nat.
+  now rewrite !retract.
+Qed.
+
+(** The typical way of proving that a type is countable is to exhibit
+    a retraction towards a known countable type. *)
+Program Definition countable_of_retract {A B} {_:Countable A} (r:Retract A B) : Countable B :=
+  Retract.compose countable (Retract.opt_lift r).
+
+
+(** * Countable instances *)
+
+Instance countable_nat : Countable nat := retract_nat_opt Retract.id.
+Instance countable_n   : Countable N := retract_nat_opt retract_nat_N.
+
+Program Instance countable_empty_set : Countable Empty_set := {|
+  inj x := 0;
+  proj x := None
+|}.
+Next Obligation.
+  intros [ [] | ].
+  reflexivity.
+Qed.
